Experiments/ProofChecking/SRChecker.lean
@@ -22,6 +22,76 @@ open LeanSAT LeanSAT.Model
 open PPA PS
 open Except
 
+
+
+-- CC: This probably shouldn't be at root, but what namespace do you put this in?
+def clauseListToPropFun (C : List ILit) : PropFun IVar :=
+  .any (Multiset.ofList C |>.map LitVar.toPropFun)
+
+def cnfListToPropFun (Cs : List (Option (List ILit))) : PropFun IVar :=
+  .all (Cs.map (fun C =>
+    match C with
+    | none => ⊤
+    | some C => clauseListToPropFun C))
+
+theorem clauseListToPropFun_eq_toPropFun (C : List ILit) :
+  clauseListToPropFun C = Clause.toPropFun ({ data := C} : IClause) := by
+  simp [clauseListToPropFun, Clause.toPropFun]
+
+-- CC: Very hacky
+theorem cnfListToPropFun_eq_toPropFun (Cs : List (Option (List ILit))) :
+  cnfListToPropFun Cs = Cnf.toPropFun ({ data := Cs.map (fun cl =>
+    match cl with
+    | none => { data := [LitVar.mkPos 1, LitVar.mkNeg 1] }
+    | some C => { data := C }) } : ICnf) := by
+  simp [cnfListToPropFun]
+  induction Cs with
+  | nil => simp
+  | cons C Cs ih =>
+    match C with
+    | none =>
+      simp [PropFun.all]
+      exact ih
+    | some C =>
+      simp
+      rw [← ih, clauseListToPropFun_eq_toPropFun]
+      simp [PropFun.all]
+
+theorem clausePropFun_ge_of_mem {C : List ILit} {l : ILit} :
+  l ∈ C → l.toPropFun ≤ clauseListToPropFun C := by
+  intro h
+  rw [clauseListToPropFun_eq_toPropFun]
+  apply Clause.toPropFun_mem_le
+  rw [← Array.mem_data]
+  exact h
+
+theorem cnfPropFun_le_of_mem {Cs : List (Option (List ILit))} {C : List ILit} {i : Nat}
+      {hi : i < Cs.length} :
+    Seq.get Cs ⟨i, hi⟩ = some C → cnfListToPropFun Cs ≤ clauseListToPropFun C := by
+  intro h
+  rw [cnfListToPropFun_eq_toPropFun]
+  induction Cs generalizing i with
+  | nil => simp at hi
+  | cons X Xs ih =>
+    match X with
+    | none =>
+      match i with
+      | 0 => simp [Seq.get] at h
+      | i + 1 =>
+        simp at hi
+        simp [Seq.get] at h
+        simp [ih h]
+    | some X =>
+      match i with
+      | 0 =>
+        simp [Seq.get] at h; subst h
+        simp [clauseListToPropFun_eq_toPropFun]
+      | i + 1 =>
+        simp [Seq.get] at h
+        have := ih h
+        apply le_trans _ this
+        simp
+
 namespace RangeArray
 
 
@@ -39,6 +109,7 @@ def uAssumeNegatedForM (F : RangeArray ILit) (τ : PPA) (bumps : Nat) : Except P
   termination_by F.usize - i
   loop 0 τ
 
+-- Returns the updated PPA. True if C is a tautology (error), false if not.
 def uAssumeNegatedFor (F : RangeArray ILit) (τ : PPA) (bumps : Nat) : PPA × Bool :=
   let usize := F.usize
   let rec loop (i : Nat) (τ : PPA) : (PPA × Bool) :=
@@ -54,9 +125,8 @@ def uAssumeNegatedFor (F : RangeArray ILit) (τ : PPA) (bumps : Nat) : PPA × Bo
   loop 0 τ
 
 -- TODO: Swap with tail-recursive function, move to PS.
-/-- Assumes into `τ` the negation of RAT clause `C` under the substitution `σ` for one "bump."
-    Errors if `C` is satisfied by either `σ` or `τ` under `σ`. -/
-def assumeRATClauseM (F : RangeArray ILit) (index : Fin F.size) (σ : PS) (τ : PPA) : Except PPA PPA :=
+/-
+def assumeRATClauseM_index (F : RangeArray ILit) (index : Fin F.size) (σ : PS) (τ : PPA) : Except PPA PPA :=
   F.foldlM_index (init := τ) (fun τ lit =>
     match σ.litValue lit with
     | Sum.inr true => error τ       -- (C|σ) is satisfied, so return early to report satisfied
@@ -65,8 +135,30 @@ def assumeRATClauseM (F : RangeArray ILit) (index : Fin F.size) (σ : PS) (τ : 
       match τ.litValue? l with
       | some true => error τ        -- (C|σ)|τ is satisfied, so return early to report satisfied
       | some false => ok τ          -- Its negation is true in τ, so ignore the literal
-      | none => ok (τ.setLit (-l))) index
+      | none => ok (τ.setLit (-l))) index -/
 
+/-- Assumes into `τ` the negation of RAT clause `C` under the substitution `σ` for one "bump."
+    Errors if `C` is satisfied by either `σ` or `τ` under `σ`. -/
+def assumeRATClauseM (F : RangeArray ILit) (index : Fin F.size) (σ : PS) (τ : PPA) : Except PPA PPA :=
+  let rsize := F.rsizeFin index
+  let rec loop (i : Nat) (τ : PPA) : Except PPA PPA :=
+    if h : i < rsize then
+      let lit := F.ogetFin index ⟨i, h⟩
+      match σ.litValue lit with
+      | Sum.inr true => error τ       -- (C|σ) is satisfied, so return early to report satisfied
+      | Sum.inr false => loop (i + 1) τ         -- Ignore the literal
+      | Sum.inl l =>
+        match τ.litValue? l with
+        | some true => error τ        -- (C|σ)|τ is satisfied, so return early to report satisfied
+        | some false => loop (i + 1) τ          -- Its negation is true in τ, so ignore the literal
+        | none => loop (i + 1) (τ.setLit (-l))
+    else
+      ok τ
+  termination_by F.rsizeFin index - i
+  loop 0 τ
+
+-- A tail-recursive implementation of `assumeRATClauseM`
+/-
 def assumeRATClause (F : RangeArray ILit) (index : Fin F.size) (σ : PS) (τ : PPA) : PPA × Bool :=
   let rsize := F.rsizeFin index
   let rec loop (i : Nat) (τ : PPA) : PPA × Bool :=
@@ -83,7 +175,28 @@ def assumeRATClause (F : RangeArray ILit) (index : Fin F.size) (σ : PS) (τ : P
     else
       ⟨τ, false⟩
   termination_by F.rsizeFin index - i
-  loop 0 τ
+  loop 0 τ -/
+
+-- A tail-recursive implementation that breaks the API to go faster
+def assumeRATClauseDirect (F : RangeArray ILit) (index : Fin F.size) (σ : PS) (τ : PPA) : Except PPA PPA :=
+  let s := F.indexFin index
+  let rsize := F.rsizeFin index
+  let e : Nat := s + rsize
+  let rec loop (i : Nat) (τ : PPA) : Except PPA PPA :=
+    if h : i < e then
+      let lit := F.getFin ⟨i, lt_of_lt_of_le h (indexFin_add_rsizeFin_le_size index)⟩
+      match σ.litValue lit with
+      | Sum.inr true => error τ
+      | Sum.inr false => loop (i + 1) τ
+      | Sum.inl l =>
+        match τ.litValue? l with
+        | some true => error τ
+        | some false => loop (i + 1) τ
+        | none => loop (i + 1) (τ.setLit (-l))
+    else
+      ok τ
+  termination_by (F.indexFin index + F.rsizeFin index) - i
+  loop s τ
 
 def unitProp (τ : PPA) (F : RangeArray ILit) (hint : Fin F.size) : PPA.UPResult :=
   let rsize := F.rsizeFin hint
@@ -106,6 +219,31 @@ def unitProp (τ : PPA) (F : RangeArray ILit) (hint : Fin F.size) : PPA.UPResult
   termination_by F.rsizeFin hint - i
   loop 0 none
 
+/-
+def unitPropDirect (τ : PPA) (F : RangeArray ILit) (hint : Fin F.size) : PPA.UPResult :=
+  let s := F.indexFin hint
+  let rsize := F.rsizeFin hint
+  let e : Nat := s + rsize
+  let he : e ≤ Size.size F.data := indexFin_add_rsizeFin_le_size hint
+  let rec loop (i : Nat) (unit? : Option ILit) : PPA.UPResult :=
+    if h : i < e then
+      let lit := F.getFin ⟨i, lt_of_lt_of_le h he⟩
+      match τ.litValue? lit with
+      | some true => .satisfied
+      | some false => loop (i + 1) unit?
+      | none =>
+        match unit? with
+        | none => loop (i + 1) (some lit)
+        | some u =>
+          if u = lit then loop (i + 1) unit?
+          else .multipleUnassignedLiterals
+    else
+      match unit? with
+      | none => .falsified
+      | some l => .unit l
+  termination_by e - i
+  loop s none -/
+
 inductive HintResult where
   | unit
   | contra
@@ -115,7 +253,7 @@ inductive HintResult where
 @[inline]
 def applyUPHint (F : RangeArray ILit) (bumps : Nat) (τ : PPA) (hint : Nat) : PPA × HintResult :=
   if h_hint : hint < F.size then
-    if !F.isDeleted hint then
+    if !F.isDeletedFin ⟨hint, h_hint⟩ then
       match unitProp τ F ⟨hint, h_hint⟩ with
       | .falsified => ⟨τ, .contra⟩
       | .satisfied =>
@@ -133,6 +271,28 @@ def applyUPHint (F : RangeArray ILit) (bumps : Nat) (τ : PPA) (hint : Nat) : PP
     -- dbg_trace s!"ERROR: Hint out of bounds"
     ⟨τ, .err⟩
 
+/-
+@[inline]
+def applyUPHintDirect (F : RangeArray ILit) (bumps : Nat) (τ : PPA) (hint : Nat) : PPA × HintResult :=
+  if h_hint : hint < F.size then
+    if !F.isDeleted hint then
+      match unitPropDirect τ F ⟨hint, h_hint⟩ with
+      | .falsified => ⟨τ, .contra⟩
+      | .satisfied =>
+        -- dbg_trace s!"ERROR: UP found a satisfied clause at index {hint}"
+        ⟨τ, .err⟩
+      | .multipleUnassignedLiterals =>
+        -- dbg_trace s!"ERROR: UP found a non-unit clause at index {hint}"
+        ⟨τ, .err⟩
+      | .unit l =>
+        -- dbg_trace s!"    Hint {hint} makes clause unit on literal {l}"
+        (τ.setLitFor l bumps, .unit)
+    else
+      ⟨τ, .err⟩
+  else
+    -- dbg_trace s!"ERROR: Hint out of bounds"
+    ⟨τ, .err⟩ -/
+
 @[inline, always_inline]
 def applyUPHints (F : RangeArray ILit) (offset : Nat) (τ : PPA) (hints : Array Nat) : PPA × HintResult :=
   let rec loop (i : Nat) (τ : PPA) : PPA × HintResult :=
@@ -144,6 +304,19 @@ def applyUPHints (F : RangeArray ILit) (offset : Nat) (τ : PPA) (hints : Array 
     else (τ, .unit)
   termination_by hints.size - i
   loop 0 τ
+
+/-
+@[inline, always_inline]
+def applyUPHintsDirect (F : RangeArray ILit) (offset : Nat) (τ : PPA) (hints : Array Nat) : PPA × HintResult :=
+  let rec loop (i : Nat) (τ : PPA) : PPA × HintResult :=
+    if hi : i < Size.size hints then
+      match applyUPHintDirect F offset τ (Seq.get hints ⟨i, hi⟩) with
+      | (τ, .unit) => loop (i + 1) τ
+      | (τ, .contra) => (τ, .contra)
+      | (τ, .err) => (τ, .err)
+    else (τ, .unit)
+  termination_by hints.size - i
+  loop 0 τ -/
 
 def reduce (σ : PS) (F : RangeArray ILit) (index : Fin F.size) : ReductionResult :=
   let rsize := F.rsizeFin index
@@ -173,6 +346,66 @@ def reduce' (σ : PS) (F : RangeArray ILit) (index : Fin F.size) : ReductionResu
       if reduced? then .reduced else .notReduced
   termination_by F.rsizeFin index - i
   loop 0 false
+
+def reduceDirect (σ : PS) (F : RangeArray ILit) (index : Fin F.size) : ReductionResult :=
+  let s := F.indexFin index
+  let rsize := F.rsizeFin index
+  let e : Nat := s + rsize
+  let he : e ≤ Size.size F.data := indexFin_add_rsizeFin_le_size index
+  let rec loop (i : Nat) (reduced? : Bool) : ReductionResult :=
+    if h : i < e then
+      let lit := F.getFin ⟨i, lt_of_lt_of_le h he⟩
+      match seval' σ lit with
+      | .satisfied => .satisfied
+      | .reduced => loop (i + 1) true
+      | .notReduced => loop (i + 1) reduced?
+    else
+      if reduced? then .reduced else .notReduced
+  termination_by e - i
+  loop s false
+
+/-
+  if hl : l.index < σ.gens.size then
+    let gen := σ.gens.get ⟨l.index, hl⟩
+    if gen ≥ σ.generation then
+      let n := σ.mappings.get ⟨l.index, by rw [σ.sizes_eq] at hl; exact hl⟩
+      match n with
+      | 0 => if polarity l then satisfied else reduced
+      | 1 => if polarity l then reduced else satisfied
+      | _ => reduced -- Technically can map to itself, but well-formed witnesses don't do this
+    else notReduced
+  else notReduced
+-/
+
+def reduceBreak (σ : PS) (F : RangeArray ILit) (index : Fin F.size) : ReductionResult :=
+  let s := F.indexFin index
+  let rsize := F.rsizeFin index
+  let e : Nat := s + rsize
+  let rec loop (i : Nat) (reduced? : Bool) : ReductionResult :=
+    if h : i < e then
+      let lit := F.getFin ⟨i, lt_of_lt_of_le h (indexFin_add_rsizeFin_le_size index)⟩
+      if hlit : lit.index < σ.gens.size then
+        let gen := σ.gens.get ⟨lit.index, hlit⟩
+        if gen ≥ σ.generation then
+          let n := σ.mappings.get ⟨lit.index, by rw [σ.sizes_eq] at hlit; exact hlit⟩
+          match n with
+          | 0 =>
+            if LitVar.polarity lit then .satisfied
+            else loop (i + 1) true
+          | 1 =>
+            if LitVar.polarity lit then loop (i + 1) true
+            else .satisfied
+          | n =>
+            if PSV.toMapped' lit ≠ n then
+              loop (i + 1) true
+            else
+              loop (i + 1) reduced?
+        else loop (i + 1) reduced?
+      else loop (i + 1) reduced?
+    else
+      if reduced? then .reduced else .notReduced
+  termination_by (F.indexFin index + F.rsizeFin index) - i
+  loop s false
 
 -- CC: Causes quadratic(?) slowdown, from 0.79 secs to 12.21 secs on php25
 --     Profiler claims that 41% of CPU is spent in σ.setLits though...
@@ -234,50 +467,46 @@ structure SRState where
   τ : PPA
   σ : PS
 
-def checkLine (st : SRState) (line : SRAdditionLine) : Except Bool SRState :=
+def checkLine : SRState → SRAdditionLine → Except Bool SRState := fun ⟨F, τ, σ⟩ line =>
   --let ⟨C, wL, wM, upHints, ratHintIndexes, ratHints, _, _⟩ := line
   -- dbg_trace s!"{C}, {wL}, {wM}"
   -- dbg_trace s!"{upHints}, {ratHintIndexes}, {ratHints}"
-  match uAssumeNegatedForM st.F st.τ.reset (line.ratHints.size + 1) with
+  match uAssumeNegatedForM F τ.reset (line.ratHints.size + 1) with
   | error _ =>
     -- dbg_trace s!"Assuming the negation of the candidate clause had error"
     error false
   | ok τ =>
-    let st := { st with τ := τ }
     -- dbg_trace s!"Assumed negation of clause succeeded"
     -- Evaluate the UP hints, with "# of RAT hints" as the offset
-    match applyUPHints st.F (line.ratHints.size + 1) st.τ line.upHints with
+    match applyUPHints F (line.ratHints.size + 1) τ line.upHints with
     | (_, .err) =>
       -- dbg_trace s!"Applying UP hints encountered an error"
       error false
     | (τ, .contra) =>
-      let st := { st with τ := τ }
       -- dbg_trace s!"Applying UP hints found contradiction before RAT"
-      if st.F.usize = 0 then error true  -- If the clause is empty, we have a successful contradiction proof
-      else ok { st with F := st.F.commit }
+      if F.usize = 0 then error true  -- If the clause is empty, we have a successful contradiction proof
+      else ok ⟨F.commit, τ, σ⟩
 
     | (τ, .unit) =>
-      let st := { st with τ := τ }
-
       -- If the clause is empty, we should have derived UP contradiction by now
-      if hu : 0 < st.F.usize then
-        let pivot : ILit := line.witnessLits.getD 0 (st.F.ugetFin ⟨0, hu⟩)
-        if pivot != st.F.ugetFin ⟨0, hu⟩ then error false else
-        let st := { st with σ := assumeWitness st.σ pivot line.witnessLits line.witnessMaps }
+      if hu : 0 < F.usize then
+        let pivot : ILit := line.witnessLits.getD 0 (F.ugetFin ⟨0, hu⟩)
+        if pivot != F.ugetFin ⟨0, hu⟩ then error false else
+        let σ := assumeWitness σ pivot line.witnessLits line.witnessMaps
 
         -- Loop through each clause in the formula to check RAT conditions
         -- The Bool is true if the check succeeds on all clauses, false otherwise
-        let Fsize := st.F.size
+        let Fsize := F.size
         let rec loop (i cachedRatHintIndex bumpCounter : Nat) (τ : PPA) : PPA × Bool :=
           if hi : i < Fsize then
-            if h_del : st.F.isDeletedFin ⟨i, hi⟩ = true then
+            if h_del : F.isDeletedFin ⟨i, hi⟩ = true then
               loop (i + 1) cachedRatHintIndex bumpCounter τ
             else
               -- First, check how the ith clause is reduced by σ
-              match reduce st.σ st.F ⟨i, hi⟩ with
+              match reduceBreak σ F ⟨i, hi⟩ with
               | .satisfied => loop (i + 1) cachedRatHintIndex bumpCounter τ
               | .notReduced => loop (i + 1) cachedRatHintIndex bumpCounter τ
-              | _ =>
+              | .reduced =>
                 -- dbg_trace s!"Clause index {i} is a RAT candidate"
                 if bumpCounter < line.ratHintIndexes.size then
                   -- Find the corresponding RAT hint
@@ -285,22 +514,534 @@ def checkLine (st : SRState) (line : SRAdditionLine) : Except Bool SRState :=
                   | none => ⟨τ, false⟩
                   | some ⟨ratIndex, hr⟩ =>
                     -- Assume the negation of the RAT clause
-                    match assumeRATClause st.F ⟨i, hi⟩ st.σ τ with
-                    | ⟨τ, true⟩ => loop (i + 1) (ratIndex + 1) (bumpCounter + 1) τ.bump
-                    | ⟨τ, false⟩ =>
-                      match applyUPHints st.F 0 τ (line.ratHints.get ⟨ratIndex, by rw [line.ratSizesEq] at hr; exact hr⟩) with
+                    match assumeRATClauseDirect F ⟨i, hi⟩ σ τ with
+                    | error τ => loop (i + 1) (ratIndex + 1) (bumpCounter + 1) τ.bump
+                    | ok τ =>
+                      match applyUPHints F 0 τ (line.ratHints.get ⟨ratIndex, by rw [line.ratSizesEq] at hr; exact hr⟩) with
                       | (τ, .unit) => ⟨τ, false⟩
                       | (τ, .contra) => loop (i + 1) (ratIndex + 1) (bumpCounter + 1) τ.bump
                       | (τ, .err) => ⟨τ, false⟩
                 else ⟨τ, false⟩
           else ⟨τ, true⟩
-        termination_by st.F.size - i
+        termination_by F.size - i
 
-        match loop 0 0 0 st.τ with
+        match loop 0 0 0 τ with
         | ⟨_, false⟩ => error false
-        | ⟨τ, true⟩ => ok { st with τ := τ, F := st.F.commit }
+        | ⟨τ, true⟩ => ok ⟨F.commit, τ, σ⟩
       else error false
 
+/-! # Correctness -/
+
+theorem uAssume.loop.aux {F : RangeArray ILit} {τ : PPA} {Ls : List (Option (List ILit))} {L : List ILit}
+  (h_models : models F Ls L) {bumps : Nat} {i j : Nat} :
+  j = Size.size L - i →
+    uAssumeNegatedForM.loop F bumps i τ = assumeNegatedClauseFor.loop { data := L } bumps i τ := by
+  intro hj
+  induction j generalizing τ i with
+  | zero =>
+    have h_le₁ := Nat.le_of_sub_eq_zero hj.symm
+    have h_le₂ := h_models.h_size₂.symm ▸ h_le₁
+    unfold assumeNegatedClauseFor.loop
+    simp only [LeanColls.size] at h_le₁ h_le₂ ⊢
+    simp [not_lt.mpr h_le₁]
+    unfold uAssumeNegatedForM.loop
+    simp [not_lt.mpr h_le₂]
+  | succ j ih =>
+    rw [Nat.succ_eq_add_one] at hj
+    unfold assumeNegatedClauseFor.loop
+    simp [LeanColls.size] at hj ⊢
+    have hi : i < List.length L := by
+      apply Nat.lt_of_sub_pos
+      rw [← hj]
+      exact Nat.zero_lt_succ j
+    simp [hi]
+    have h_silly : Seq.get ({ data := L} : IClause) ⟨i, hi⟩ = Seq.get L ⟨i, hi⟩ := rfl
+    have h_agree := h_models.h_uncommitted hi
+    split <;> rename _ => h_get
+    · rw [← @ih (setLitFor τ (-Seq.get ({ data := L} : IClause) { val := i, isLt := hi }) bumps) (i + 1)]
+      · rw [uAssumeNegatedForM.loop]
+        rw [h_silly, ← h_agree] at h_get
+        have := h_models.h_size₂
+        simp [LeanColls.size] at this
+        rw [← this] at hi
+        simp [hi]
+        simp [ugetFin_eq_uget, h_get]
+        rw [h_agree]
+        rfl
+      · simp [LeanColls.size]; exact Nat.eq_sub_succ_of_succ_eq_sub hj
+    · rw [← @ih τ]
+      rw [uAssumeNegatedForM.loop]
+      split <;> rename _ => hi'
+      · simp [ugetFin_eq_uget, h_agree, ← h_silly, h_get]
+      · rw [h_models.h_size₂] at hi'
+        exact absurd hi hi'
+      · simp [LeanColls.size]; exact Nat.eq_sub_succ_of_succ_eq_sub hj
+    · rw [uAssumeNegatedForM.loop]
+      split <;> rename _ => hi'
+      · simp [ugetFin_eq_uget, h_agree, ← h_silly, h_get]
+      · rw [h_models.h_size₂] at hi'
+        exact absurd hi hi'
+
+theorem uAssumeNegatedForM_eq_assumeNegatedClauseFor {F : RangeArray ILit}
+    {Ls : List (Option (List ILit))} {L : List ILit} {τ : PPA} {bumps : Nat} :
+    models F Ls L →
+    uAssumeNegatedForM F τ bumps = assumeNegatedClauseFor τ ({ data := L} : IClause) bumps := by
+  intro h_models
+  simp [uAssumeNegatedForM, assumeNegatedClauseFor]
+  rw [@uAssume.loop.aux _ _ _ _ h_models bumps 0 (Size.size L)]
+  simp
+
+theorem assumeRATClauseDirect.loop.aux {F : RangeArray ILit} {Ls : List (Option (List ILit))} {L : List ILit}
+  (h_models : models F Ls L) {σ : PS} {i j : Nat} (hi : i < F.size) :
+  --    k = F.rsizeFin ⟨i, hi⟩ - j
+    j = F.rsizeFin ⟨i, hi⟩ - i →
+    assumeRATClauseDirect.loop F i σ j = assumeRATClauseM F hint σ := by
+  intro hj
+  induction j generalizing σ i with
+  | zero =>
+    have h_le₁ := Nat.le_of_sub_eq_zero hj.symm
+    have h_le₂ := h_models.h_size₂.symm ▸ h_le₁
+    unfold assumeRATClauseM
+    simp [not_lt.mpr h_le₂]
+    unfold assumeRATClauseDirect
+    simp [not_lt.mpr h_le₁]
+  | succ j ih =>
+    rw [Nat.succ_eq_add_one] at hj
+    unfold assumeRATClauseM
+    simp [LeanColls.size] at hj ⊢
+    have hi : i < List.length L := by
+      apply Nat.lt_of_sub_pos
+      rw [← hj]
+      exact Nat.zero_lt_succ j
+    simp [hi]
+    have h_silly : Seq.get ({ data := L} : IClause) ⟨i, hi⟩ = Seq.get L ⟨i, hi⟩ := rfl
+    have h_agree := h_models.h_uncommitted hi
+    split <;> rename _ => h_get
+    · rw [← @ih (σ.setLit (-Seq.get ({ data := L} : IClause) { val := i, isLt := hi })) (i + 1)]
+      · rw [assumeRATClauseDirect.loop]
+        rw [h_silly, ← h_agree] at h_get
+        have := h_models.h_size₂
+        simp [LeanColls.size] at this
+        rw [← this] at hi
+        simp [hi]
+        simp [ogetFin_eq_oget, h_get]
+        rw [h_agree]
+        rfl
+      · simp [LeanColls.size]; exact Nat.eq_sub_succ_of_succ_eq_sub hj
+    · rw [← @ih σ]
+      rw [assumeRATClauseDirect.loop]
+      split <;> rename _ => hi'
+      · simp [ogetFin_eq_oget, h_agree
+
+#exit
+
+theorem RangeArray.unitProp_eq_unitProp {F : RangeArray ILit}
+  {Ls : List (Option (List ILit))} {L C : List ILit} (h_models : models F Ls L)
+  {τ : PPA} {hint : Nat} {h_hint : hint < Size.size Ls} :
+    Seq.get Ls ⟨hint, h_hint⟩ = some C →
+    RangeArray.unitProp τ F ⟨hint, h_models.h_size₁ ▸ h_hint⟩ = PPA.unitProp τ ({ data := C } : IClause) := by
+  sorry
+  done
+
+-- Clone of PPA.LawfulUP, but with `RangeArray`
+theorem applyUPHint_unit {F : RangeArray ILit} {Ls : List (Option (List ILit))} {L : List ILit}
+    (h_models : models F Ls L) {τ τ' : PPA} {bumps : Nat} {hint : Nat} :
+    applyUPHint F bumps τ hint = (τ', .unit) →
+      (h_hint : hint < Size.size Ls) ×'
+      ∃ (C : List ILit), Seq.get Ls ⟨hint, h_hint⟩ = some C ∧
+        ∃ (l : ILit),
+          l ∈ C ∧
+          τ.litValue? l = none ∧
+          τ' = τ.setLitFor l bumps ∧ (clauseListToPropFun C) ⊓ τ = l.toPropFun ⊓ τ ∧
+          (cnfListToPropFun Ls) ⊓ τ ≤ τ' := by
+  simp [applyUPHint]
+  intro h
+  by_cases h_hint : hint < F.size
+  <;> simp [h_hint] at h
+  by_cases h_del : isDeletedFin F ⟨hint, h_hint⟩
+  <;> simp [h_del] at h
+  split at h
+  <;> injection h <;> try contradiction
+  rename ILit => lit
+  rename _ = UPResult.unit lit => h_up
+  rename setLitFor τ lit bumps = _ => h_set
+  subst h_set
+  have h_hint₂ := h_models.h_size₁ ▸ h_hint
+  use h_hint₂
+  simp at h_del
+  rw [isDeletedFin_eq_isDeleted h_hint] at h_del
+  rcases get_eq_some_of_models_of_not_deleted h_models h_del with ⟨_, sL, hsL⟩
+  use sL, hsL
+  rw [RangeArray.unitProp_eq_unitProp h_models hsL] at h_up
+  have := (unitProp_LawfulUP τ ({ data := sL } : IClause)).2.1 h_up
+  rcases this with ⟨h_lit_mem, h₁, h₂⟩
+  simp [← Array.mem_data] at h_lit_mem
+  simp [clauseListToPropFun_eq_toPropFun]
+  use lit, h_lit_mem, h₁, rfl, h₂
+  simp [toPropFun_setLit_of_none h₁]
+  have := cnfPropFun_le_of_mem hsL
+  apply le_trans (inf_le_inf_right τ.toPropFun this)
+  rw [clauseListToPropFun_eq_toPropFun, h₂]
+  exact inf_le_left
+
+theorem applyUPHint_contra {F : RangeArray ILit} {Ls : List (Option (List ILit))} {L : List ILit}
+    (h_models : models F Ls L) {τ τ' : PPA} {bumps : Nat} {hint : Nat} :
+    (applyUPHint F bumps τ hint = (τ', .contra) →
+      (h_hint : hint < Size.size Ls) ×'
+      ∃ (C : List ILit), Seq.get Ls ⟨hint, h_hint⟩ = some C
+        ∧ τ = τ' ∧ (clauseListToPropFun C) ⊓ τ = ⊥) := by
+  simp [applyUPHint]
+  intro h
+  by_cases h_hint : hint < F.size
+  <;> simp [h_hint] at h
+  by_cases h_del : isDeletedFin F ⟨hint, h_hint⟩
+  <;> simp [h_del] at h
+  split at h
+  <;> injection h <;> try contradiction
+  rename τ = _ => hτ; subst hτ
+  simp at h_del
+  rw [isDeletedFin_eq_isDeleted h_hint] at h_del
+  have := lt_of_isDeleted_false h_del
+  use h_models.h_size₁ ▸ this
+  rcases get_eq_some_of_models_of_not_deleted h_models h_del with ⟨_, sL, hsL⟩
+  use sL, hsL, rfl
+  rename _ = UPResult.falsified => h_up
+  rw [RangeArray.unitProp_eq_unitProp h_models hsL] at h_up
+  rw [clauseListToPropFun_eq_toPropFun]
+  exact (unitProp_LawfulUP τ ({ data := sL } : IClause)).1 h_up
+
+-- CC: Clone of proof from `unitProp.go.cons_aux`
+theorem applyUPHints.loop.cons_aux (F : RangeArray ILit) (τ : PPA) (bumps : Nat)
+    (hint : Nat) {hints : List Nat} {i j : Nat} :
+    j = Size.size hints - i → applyUPHints.loop F bumps { data := hint :: hints } (i + 1) τ =
+      applyUPHints.loop F bumps { data := hints } i τ := by
+  intro hj
+  induction j generalizing τ i with
+  | zero =>
+    have : i ≥ LeanColls.size hints := Nat.le_of_sub_eq_zero hj.symm
+    unfold applyUPHints.loop
+    simp [LeanColls.size] at this ⊢
+    simp [not_lt.mpr this, not_lt.mpr (Nat.succ_le_succ_iff.mpr this)]
+  | succ j ih =>
+    unfold applyUPHints.loop
+    simp [LeanColls.size, Nat.succ_eq_add_one] at hj ⊢
+    have hi : i < List.length hints := by
+      apply Nat.lt_of_sub_pos
+      rw [← hj]
+      exact Nat.zero_lt_succ j
+    simp [hi]
+    have : Seq.get ({data := hint :: hints} : Array Nat) ⟨i + 1, Nat.succ_lt_succ hi⟩
+      = Seq.get ({data := hints} : Array Nat) ⟨i, hi⟩ := rfl
+    rw [this]
+    split <;> rename PPA => τ' <;> rename _ => h_up
+    <;> simp [h_up]
+    apply ih
+    simp [LeanColls.size]
+    exact Nat.eq_sub_succ_of_succ_eq_sub hj
+
+theorem applyUPHints.loop.cons (F : RangeArray ILit) (τ : PPA) (bumps : Nat)
+    (hint : Nat) (hints : List Nat) (i : Nat) :
+    applyUPHints.loop F bumps { data := hint :: hints } (i + 1) τ =
+      applyUPHints.loop F bumps { data := hints } i τ :=
+  @applyUPHints.loop.cons_aux F τ bumps hint hints i (hints.length - i) rfl
+
+theorem applyUPHints_unit {F : RangeArray ILit} {Ls : List (Option (List ILit))} {L : List ILit}
+    (h_models : models F Ls L) {τ τ' : PPA} {bumps : Nat} {hints : Array Nat} :
+    applyUPHints F bumps τ hints = (τ', .unit) →
+      (cnfListToPropFun Ls) ⊓ τ ≤ τ' ∧ extended τ τ' bumps := by
+  have ⟨hints⟩ := hints
+  rw [applyUPHints] --, applyUPHints.loop]
+  induction hints generalizing τ τ' with
+  | nil =>
+    rw [applyUPHints.loop]
+    simp [LeanColls.size]
+    rintro rfl
+    constructor
+    · exact inf_le_right
+    · simp
+  | cons hint hints ih =>
+    intro h_uphints
+    rw [applyUPHints.loop] at h_uphints
+    simp [LeanColls.size] at h_uphints
+    split at h_uphints
+    <;> rename PPA => τ₂
+    · rename applyUPHint _ _ _ _ = _ => h_up
+      rw [applyUPHints.loop.cons] at h_uphints
+      rcases applyUPHint_unit h_models h_up with ⟨h_hint, sL, _, lit', _, hτlit', rfl, _, h_inf₂⟩
+      rcases ih h_uphints with ⟨h₁, h₂⟩
+      have h_ext := extended_setLitFor_of_none hτlit' bumps
+      constructor
+      · have := entails_of_extended h₂
+        have h_toPropFun := toPropFun_setLit_of_none hτlit'
+        simp [h_toPropFun] at this
+        have := inf_le_inf_left (cnfListToPropFun Ls) h_inf₂
+        rw [← inf_assoc, inf_idem] at this
+        exact le_trans this h₁
+      · exact extended_trans h_ext h₂
+    · injection h_uphints
+      contradiction
+    · injection h_uphints
+      contradiction
+
+theorem applyUPHints_contra {F : RangeArray ILit} {Ls : List (Option (List ILit))} {L : List ILit}
+    (h_models : models F Ls L) {τ τ' : PPA} {bumps : Nat} {hints : Array Nat} :
+    applyUPHints F bumps τ hints = (τ', .contra) →
+      (cnfListToPropFun Ls) ⊓ τ = ⊥ ∧ extended τ τ' bumps := by
+  have ⟨hints⟩ := hints
+  rw [applyUPHints]
+  induction hints generalizing τ τ' with
+  | nil =>
+    rw [applyUPHints.loop]
+    simp [LeanColls.size]
+  | cons hint hints ih =>
+    intro h_uphints
+    rw [applyUPHints.loop] at h_uphints
+    simp [LeanColls.size] at h_uphints
+    split at h_uphints
+    <;> rename PPA => τ₂
+    · rename applyUPHint _ _ _ _ = _ => h_up
+      rw [applyUPHints.loop.cons] at h_uphints
+      rcases applyUPHint_unit h_models h_up with ⟨h_hint, sL, _, lit', _, hτlit', rfl, _, h_inf₂⟩
+      rcases ih h_uphints with ⟨h₁, h₂⟩
+      constructor
+      · simp at h₁ h_inf₂
+        have h_toPropFun := toPropFun_setLit_of_none hτlit'
+        rw [h_toPropFun] at h₁ h_inf₂
+        rw [← inf_assoc] at h₁
+        have := inf_le_inf_left (cnfListToPropFun Ls) h_inf₂
+        simp_rw [← inf_assoc, inf_idem] at this
+        rw [eq_bot_iff] at h₁ ⊢
+        exact le_trans this h₁
+      · exact extended_trans (extended_setLitFor_of_none hτlit' bumps) h₂
+    · injection h_uphints
+      rename τ₂ = _ => h; subst h
+      rename applyUPHint _ _ _ _ = _ => h_up
+      rcases applyUPHint_contra h_models h_up with ⟨h_hint, sL, hsL, rfl, h_inf⟩
+      constructor
+      · have := cnfPropFun_le_of_mem hsL
+        rw [eq_bot_iff] at h_inf ⊢
+        have := inf_le_inf_right τ.toPropFun this
+        exact le_trans this h_inf
+      · exact extended_refl _ _
+    · injection h_uphints; contradiction
+
+theorem reduce_eq_reduce {F : RangeArray ILit} {Ls : List (Option (List ILit))} {L : List ILit}
+    (h_models : models F Ls L) {C : List ILit}
+    {i : Nat} (hi : i < Size.size Ls) :
+    Seq.get Ls ⟨i, hi⟩ = some C →
+      ∀ (σ : PS), RangeArray.reduce σ F ⟨i, h_models.h_size₁ ▸ hi⟩ = PS.reduce σ ({ data := C} : IClause) := by
+  sorry
+  done
+
+theorem reduceBreak.loop_eq_reduce.loop_aux {F : RangeArray ILit} {i : Nat} {hi : i < F.size}
+    (σ : PS) {j k : Nat} :
+    k = F.rsizeFin ⟨i, hi⟩ - j →
+      reduceBreak.loop σ F ⟨i, hi⟩ (F.indexFin ⟨i, hi⟩ + j) = RangeArray.reduce.loop σ F ⟨i, hi⟩ j := by
+  intro hk
+  ext reduced?
+  induction k generalizing σ j reduced? with
+  | zero =>
+    have h_le := Nat.le_of_sub_eq_zero hk.symm
+    unfold reduceBreak.loop RangeArray.reduce.loop
+    simp [Nat.not_lt.mpr h_le]
+  | succ k ih =>
+    have := ih σ (Nat.eq_sub_succ_of_succ_eq_sub hk)
+    unfold reduceBreak.loop RangeArray.reduce.loop
+    have hj : j < F.rsizeFin ⟨i, hi⟩ := by
+      apply Nat.lt_of_sub_pos
+      rw [← hk]
+      exact Nat.zero_lt_succ k
+    simp [hj, seval', litValue, ogetFin, varValue]
+    split
+    · rename _ => h_lit
+      have h_var := h_lit
+      simp [ILit.index, σ.sizes_eq] at h_var
+      split
+      · rename _ => h_gen
+        split
+        <;> rename _ => h_mappings
+        <;> simp [ILit.index] at h_mappings
+        <;> simp [h_mappings]
+        · split
+          · rfl
+          · exact this true
+        · split
+          · exact this true
+          · rfl
+        · rename _ = 0 → False => h_ne_0
+          rename _ = 1 → False => h_ne_1
+          split
+          · exact this reduced?
+          · exact this true
+      · exact this reduced?
+    · exact this reduced?
+
+theorem reduceBreak.loop_eq_reduce.loop (F : RangeArray ILit) {i : Nat} (hi : i < F.size) (σ : PS) :
+    reduceBreak.loop σ F ⟨i, hi⟩ (F.indexFin ⟨i, hi⟩) = RangeArray.reduce.loop σ F ⟨i, hi⟩ 0 :=
+  @reduceBreak.loop_eq_reduce.loop_aux F i hi σ 0 (F.rsizeFin ⟨i, hi⟩) rfl
+
+theorem reduceBreak_eq_reduce (F : RangeArray ILit) {i : Nat} (hi : i < F.size) (σ : PS) :
+    RangeArray.reduceBreak σ F ⟨i, hi⟩ = RangeArray.reduce σ F ⟨i, hi⟩ := by
+  unfold reduceBreak RangeArray.reduce
+  simp [reduceBreak.loop_eq_reduce.loop F hi]
+
+theorem checkLine.loop_ok {line : SRAdditionLine} {F : RangeArray ILit} {Ls : List (Option (List ILit))} {L : List ILit}
+    (h_models : models F Ls L) {τ τ' : PPA} {σ : PS} {i j cri bc : Nat} :
+  j = F.size - i →
+  uniform τ (numRatHints - bc) →
+    checkLine.loop line F σ i cri bc τ = ⟨τ', true⟩ →
+      (τ = τ' ∨ uniform τ' (numRatHints - (bc + 1)))
+      ∧ τ'.toPropFun = τ.toPropFun
+      ∧ ∀ (k : Nat) (hk₁ : k ≥ i) (hk₂ : k < Size.size Ls) (C : List ILit),
+        Seq.get Ls ⟨k, hk₂⟩ = some C →
+          (clauseListToPropFun C) ⊓ τ ≤ PropFun.substL (clauseListToPropFun C) σ.toSubst := by
+  intro hj h_uniform
+  induction j generalizing τ i cri bc with
+  | zero =>
+    have hi : i ≥ F.size := Nat.le_of_sub_eq_zero hj.symm
+    unfold loop
+    simp [not_lt.mpr hi, not_lt.mpr (Nat.succ_le_succ_iff.mpr hi)]
+    rintro rfl
+    simp
+    intro k hk₁ hk₂
+    rw [← h_models.h_size₁] at hk₂
+    have := lt_of_le_of_lt hk₁ hk₂
+    exact absurd this (not_lt.mpr hi)
+  | succ j ih =>
+    unfold loop
+    have hi : i < F.size := by
+      apply Nat.lt_of_sub_pos
+      rw [← hj]
+      exact Nat.zero_lt_succ j
+    simp [hi]
+    -- Split on whether the ith clause is deleted
+    split
+    · -- Deleted, so we skip the clause
+      rename _ = true => h_del
+      intro h_loop
+      rcases ih (Nat.eq_sub_succ_of_succ_eq_sub hj) h_uniform h_loop with ⟨hτ, hpf, hkC⟩
+      use hτ, hpf
+      intro k hk₁ hk₂ C hC
+      rw [isDeletedFin_eq_isDeleted hi] at h_del
+      by_cases hik : i = k
+      · -- if i = k, then we derive contradiction
+        subst hik
+        rw [h_models.h_size₁] at hi
+        have := h_models.h_some hi
+        simp [h_del, hC] at this
+      · -- Otherwise, k is a higher index
+        have : i + 1 ≤ k := Nat.succ_le_of_lt (lt_of_le_of_ne hk₁ hik)
+        exact hkC _ this hk₂ C hC
+    · -- Not deleted, so we actually check the clause
+      rename ¬(_ = true) => h_del; simp at h_del
+      split
+      · -- Reduction returned .satisfied
+        rename _ => h_reducedSatisfied
+        intro h_loop
+        rcases ih (Nat.eq_sub_succ_of_succ_eq_sub hj) h_uniform h_loop with ⟨hτ, hpf, hkC⟩
+        use hτ, hpf
+        intro k hk₁ hk₂ C hC
+        have hj' := Nat.eq_sub_succ_of_succ_eq_sub hj
+        by_cases hik : i = k
+        · -- if i = k, then the loop body checks the kth clause
+          subst hik
+          rw [reduceBreak_eq_reduce F hi σ] at h_reducedSatisfied
+          rw [h_models.h_size₁] at hi
+          rw [reduce_eq_reduce h_models hi hC] at h_reducedSatisfied
+          rw [clauseListToPropFun_eq_toPropFun]
+          simp [(PS.reduce_Lawful σ { data := C }).1 h_reducedSatisfied]
+        · -- Otherwise, k is a higher index
+          have : i + 1 ≤ k := Nat.succ_le_of_lt (lt_of_le_of_ne hk₁ hik)
+          exact hkC _ this hk₂ C hC
+      · -- Reduction returned .notReduced, so we skip the clause here too
+        rename _ => h_notReduced
+        intro h_loop
+        rcases ih (Nat.eq_sub_succ_of_succ_eq_sub hj) h_uniform h_loop with ⟨hτ, hpf, hkC⟩
+        use hτ, hpf
+        intro k hk₁ hk₂ C hC
+        have hj' := Nat.eq_sub_succ_of_succ_eq_sub hj
+        by_cases hik : i = k
+        · -- if i = k, then the loop body checks the kth clause
+          subst hik
+          rw [reduceBreak_eq_reduce F hi σ] at h_notReduced
+          rw [h_models.h_size₁] at hi
+          rw [reduce_eq_reduce h_models hi hC] at h_notReduced
+          rw [clauseListToPropFun_eq_toPropFun]
+          simp [(PS.reduce_Lawful σ { data := C }).2 h_notReduced]
+        · -- Otherwise, k is a higher index
+          have : i + 1 ≤ k := Nat.succ_le_of_lt (lt_of_le_of_ne hk₁ hik)
+          exact hkC _ this hk₂ C hC
+      · -- Reduction returned .reduced
+        rename _ => h_reduced
+        split <;> try simp
+        rename bc < _ => h_bc
+        split <;> try simp
+        rename Nat => ratIndex
+        rename ratIndex < _ => h_ratIndex
+        rename _ => h_findRatHint
+        -- How does assuming the negation of the reduced clause go?
+        split
+        · rename PPA => τ₂
+          rename _ => h_assumeRAT
+          --rw [assumeRATClauseDirect_eq_assumeRATClauseDirectFor h_models h_reduced]
+          intro h_loop
+          rcases ih (Nat.eq_sub_succ_of_succ_eq_sub hj) h_loop with ⟨hτ, hpf, hkC⟩
+          ·
+            done
+          done
+        done
+      done
+    done
+  done
+
+#exit
+
+theorem checkLine_correct {F : RangeArray ILit} {τ : PPA} {σ : PS} {line : SRAdditionLine}
+    {S : SRState} {Cs : List (Option (List ILit))} {C : List ILit} :
+    models F Cs C →
+    checkLine ⟨F, τ, σ⟩ line = .ok S →
+    -- S = ⟨F.commit, τ', σ'⟩ ∧
+    PropFun.eqsat (cnfListToPropFun Cs) (cnfListToPropFun Cs ⊓ clauseListToPropFun C) := by
+  intro h_models h_checkLine
+  simp [checkLine] at h_checkLine
+  split at h_checkLine
+  · contradiction
+  · rename PPA => τ₁
+    rename _ = ok τ₁ => h_uAssume
+    rw [uAssumeNegatedForM_eq_assumeNegatedClauseFor h_models] at h_uAssume
+    rcases PPA.assumeNegatedClauseFor_Lawful τ.reset τ₁ { data := C } (Array.size line.ratHints + 1) with ⟨_, h₂⟩
+    rcases h₂ h_uAssume with ⟨h_toPropFun_τ₁, h_ext_τ₁⟩
+    simp at h_toPropFun_τ₁
+    clear h₂
+    split at h_checkLine
+    <;> rename PPA => τ₂
+    · contradiction
+    · split at h_checkLine
+      · contradiction
+      · injection h_checkLine
+        rename _ = (_, HintResult.contra) => h_hints
+        rcases applyUPHints_contra h_models h_hints with ⟨hF, _⟩
+        rw [h_toPropFun_τ₁] at hF
+        apply PropFun.eqsat_of_entails
+        rw [clauseListToPropFun_eq_toPropFun]
+        rwa [eq_bot_iff, ← PropFun.le_iff_inf_compl_le_bot] at hF
+    · split at h_checkLine <;> try contradiction
+      rename applyUPHints _ _ _ _ = _ => h_uphints
+      rename F.dsize < _ => h_Fsize
+      split at h_checkLine <;> try contradiction
+      rename _ = ugetFin _ => h_getD
+      split at h_checkLine <;> try contradiction
+      rename PPA => τ₃
+      rename checkLine.loop _ _ _ _ _ _ _ = _ => h_checkLine_loop
+      injection h_checkLine; rename _ => hS
+
+      stop
+      done
+
+    done
+  done
+
+#exit
 /-def checkLine (F : RangeArray ILit) (τ : PPA) (σ : PS) (line : SRAdditionLine)
     : Except Bool (RangeArray ILit × PPA × PS) :=
   --let ⟨C, wL, wM, upHints, ratHintIndexes, ratHints, _, _⟩ := line
